src/slf/WPsem.v
@@ -5,7 +5,8 @@ From SLF Require Export Rules.
 
 Implicit Types f : var.
 Implicit Types b : bool.
-Implicit Types v : val.
+Implicit Types v w : val.
+Implicit Types p : loc.
 Implicit Types h : heap.
 Implicit Types P : Prop.
 Implicit Types H : hprop.
@@ -14,21 +15,18 @@ Implicit Types Q : val->hprop.
 (* ################################################################# *)
 (** * First Pass *)
 
-(** In previous chapters, we have introduced the notion of
-    Separation Logic triple, written [triple t H Q].
+(** In previous chapters, we have introduced the notion of Separation Logic
+    triple, written [triple t H Q]. In this chapter, we introduce the notion of
+    "weakest precondition" for Separation Logic triples, written [wp t Q]. The
+    intention is for [wp t Q] to be a heap predicate (of type [hprop]) such that
+    [H ==> wp t Q] if and only if [triple t H Q] holds.
 
-    In this chapter, we introduce the notion of "weakest precondition"
-    for Separation Logic triples, written [wp t Q].
+    The benefits of introducing weakest preconditions is two-fold.
 
-    The intention is for [wp t Q] to be a heap predicate (of type [hprop])
-    such that [H ==> wp t Q] if and only if [triple t H Q] holds.
-
-    The benefits of introducing weakest preconditions is two-fold:
-
-    - the use of [wp] greatly reduces the number of structural rules
+    - The use of [wp] greatly reduces the number of structural rules
       required, and thus reduces accordingly the number of tactics
       required for carrying out proofs in practice;
-    - the predicate [wp] will serve as guidelines for setting up in the
+    - The predicate [wp] will serve as guidelines for setting up in the
       next chapter a "characteristic formula generator", which is the
       key ingredient at the heart of the implementation of the CFML tool.
 
@@ -37,125 +35,144 @@ Implicit Types Q : val->hprop.
     - the notion of weakest precondition, as captured by [wp],
     - the reformulation of structural rules in [wp]-style,
     - the reformulation of reasoning rules in [wp]-style,
-    - (optional) alternative, equivalent definitions for [wp],
-      and alternative proofs for deriving [wp]-style reasoning rules. *)
+
+    The "optional material" section presents several equivalent definitions for
+    [wp], alternative proofs for deriving [wp]-style reasoning rules, as well as
+    a presentation of "Texan triples", which reformulate function specifications
+    using magic wands instead of triples. *)
 
 (* ================================================================= *)
 (** ** Notion of Weakest Precondition *)
 
-(** We next introduce a function [wp], called "weakest precondition".
-    Given a term [t] and a postcondition [Q], the expression [wp t Q]
-    denotes a heap predicate [wp t Q] such that, for any heap predicate
-    [H], the entailment [H ==> wp t Q] is equivalent to [triple t H Q].
+(** Consider a term [t] and a postcondition [Q]. The expression [wp t Q] is
+    called the "weakest precondition" of the term [t] with respect to the
+    postcondition [Q]. This weakest precondition consists of a heap predicate
+    such that, for any heap predicate [H], the entailment [H ==> wp t Q] holds
+    if and only if [triple t H Q] holds. The notion of [wp] might sound very
+    mysterious at this point. Hopefully, it will become clearer through the
+    reading of this chapter. *)
 
-    The notion of [wp] usually sounds fairly mysterious at first sight.
-    It will make more sense when we describe the properties of [wp]. *)
+(** The first critical observation is that [wp] is in fact nothing but a mere
+    reformulation of the predicate [eval]. To see why, recall the definition of
+    [triple t H Q].
 
-Parameter wp : trm -> (val->hprop) -> hprop.
+    Definition triple (t:trm) (H:hprop) (Q:val->hprop) : Prop :=
+      forall s, H s -> eval s t Q.
 
-Parameter wp_equiv : forall t H Q,
+By definition, the predicate [wp] should be such that [H ==> wp t Q] is
+equivalent to [triple t H Q]. But [H ==> wp t Q] unfolds to
+[forall s, H s -> wp t Q s]. If we compare [forall s, H s -> eval s t Q] with
+[forall s, H s -> wp t Q s], we see that [wp t Q s] should match [eval s t Q].
+In other words, [wp t Q] should correspond to [fun s => eval s t Q]. *)
+
+Definition wp (t : trm) (Q : val->hprop) : hprop :=
+  fun s => eval s t Q.
+
+Lemma wp_equiv : forall t H Q,
   (H ==> wp t Q) <-> (triple t H Q).
+Proof using.
+  iff M. { introv Hs. applys M Hs. } { introv Hs. applys M Hs. }
+Qed.
 
-(** The [wp t Q] is called "weakest precondition" for two reasons:
-    because (1) it is a precondition, and (2) it is the weakest one,
-    as we explain next.
+(** There exists several other ways of defining [wp]. As we show near the end of
+    this chapter, they are all equivalent. The definition considered above is
+    the one that leads to the simplest proofs for the reasoning rules. Indeed,
+    reasoning rules must be proved correct with respect to the semantics, and
+    the semantics is captured by the predicate [eval]. *)
 
-    First, [wp t Q] is always a "valid precondition" for a
-    triple associated with the term [t] and the postcondition [Q]. *)
+(** Let us now explain why [wp] is called a "weakest precondition". First,
+    [wp t Q] is always a "valid precondition" for a triple associated with the
+    term [t] and the postcondition [Q]. *)
 
 Lemma wp_pre : forall t Q,
   triple t (wp t Q) Q.
 Proof using. intros. rewrite <- wp_equiv. applys himpl_refl. Qed.
 
-(** Second, [wp t Q] is the "weakest" of all valid preconditions
-    for the term [t] and the postcondition [Q], in the sense that
-    any other valid precondition [H], i.e. satisfying [triple t H Q],
-    is such that [H] entails [wp t Q]. *)
+(** Second, [wp t Q] is the "weakest" of all valid preconditions for the term
+    [t] and the postcondition [Q], in the sense that, for any other valid
+    precondition [H] (i.e., such that [triple t H Q] holds), it is the case that
+    [H] entails [wp t Q]. *)
 
 Lemma wp_weakest : forall t H Q,
   triple t H Q ->
   H ==> wp t Q.
 Proof using. introv M. rewrite wp_equiv. applys M. Qed.
 
-(** There are several equivalent ways to define [wp], as we show
-    in the optional contents of this chapter. It turns out that
-    the equivalence [(H ==> wp t Q) <-> (triple t H Q)] fully
-    characterizes the predicate [wp], and that it is all we need
-    to carry out formal reasoning.
-
-    For this reason, we postpone to further on in this chapter the
-    description of alternative, direct definitions for [wp]. *)
-
 (* ================================================================= *)
 (** ** Structural Rules in Weakest-Precondition Style *)
 
-(** We next present reformulations of the frame rule and of the rule
-    of consequence in "weakest-precondition style". *)
+(** We next present reformulations of the frame rule and of the rule of
+    consequence in "weakest-precondition style". Thereafter, given a term [t]
+    and a postcondition [Q], we say that "[t] produces [Q]" if [t] terminates
+    and produces a output value and an output state that, together, satisfy the
+    postcondition [Q]. *)
 
 (* ----------------------------------------------------------------- *)
 (** *** The Frame Rule *)
 
 (** The frame rule for [wp] asserts that [(wp t Q) \* H] entails
-    [wp t (Q \*+ H)]. This statement can be read as follows:
-    if you own both a piece of state satisfying [H] and a piece of state
-    in which the execution of [t] produces (a result and an output value
-    satisfying) [Q], then you own a piece of state in which the execution
-    of [t] produces [Q \*+ H], that is, produces both [Q] and [H]. *)
+    [wp t (Q \*+ H)]. This statement can be read as follows: if you own both a
+    piece of state satisfying [H] and a piece of state in which the execution of
+    [t] produces [Q], then you own a piece of state in which the execution of
+    [t] produces [Q \*+ H], that is, produces both [Q] and [H]. *)
 
 Lemma wp_frame : forall t H Q,
   (wp t Q) \* H ==> wp t (Q \*+ H).
 
-(** The lemma is proved by exploiting the frame rule for triples
-    and the equivalence that characterizes [wp]. *)
+(** The lemma is proved by exploiting the frame property on [eval]. (It could
+    also be derived using [wp_equiv] and [triple_frame], but the point here is
+    to derive properties of [wp] without involving [triple].) *)
 
 Proof using.
-  intros. rewrite wp_equiv.
-  applys triple_frame. rewrite* <- wp_equiv.
+  intros. unfold wp. intros h HF.
+  lets (h1&h2&M1&M2&MD&MU): hstar_inv (rm HF).
+  subst. applys eval_conseq.
+  { applys eval_frame M1 MD. }
+  { xsimpl. intros h' ->. applys M2. }
 Qed.
 
-(** The connection with the frame might not be totally obvious.
-    Recall the frame rule for triples.
+(** The connection with the frame rule for triples might not be totally obvious.
+    Recall the statement of the frame rule.
 
     triple t H1 Q ->
     triple t (H1 \* H) (Q \*+ H)
 
-    Let us replace the form [triple t H Q] with the form
-    [H ==> wp t Q]. We obtain the following statement. *)
+    Let us replace the pattern [triple t H Q] with the pattern [H ==> wp t Q],
+    following the characteristic equivalence [wp_equiv]. We obtain the statement
+    shown below. *)
 
 Lemma wp_frame_trans : forall t H1 Q H,
   H1 ==> wp t Q ->
   (H1 \* H) ==> wp t (Q \*+ H).
 
-(** If we exploit transitivity of entailment to eliminate [H1], then we
-    obtain exactly [wp_frame], as illustrated by the proof script below. *)
+(** If we exploit transitivity of entailment to eliminate [H1], then we obtain
+    exactly [wp_frame], as illustrated by the proof script below. *)
 
 Proof using. introv M. xchange M. applys* wp_frame. Qed.
 
 (* ----------------------------------------------------------------- *)
 (** *** The Rule of Consequence *)
 
-(** The rule of consequence for [wp] materializes as a covariance
-    property: it asserts that [wp t Q] is covariant in [Q].
-    In other words, if one weakens [Q], then one weakens [wp t Q].
-    The corresponding formal statement appears next. *)
+(** The rule of consequence for [wp] materializes as a covariance property: it
+    asserts that [wp t Q] is covariant in [Q]. In other words, if [Q1] entails
+    [Q2], then [wp t Q1] entails [wp t Q2]. The corresponding formal statement
+    appears next. *)
 
 Lemma wp_conseq : forall t Q1 Q2,
   Q1 ===> Q2 ->
   wp t Q1 ==> wp t Q2.
-Proof using.
-  introv M. rewrite wp_equiv. applys* triple_conseq (wp t Q1) M. applys wp_pre.
-Qed.
+Proof using. unfold wp. introv M. intros s Hs. applys* eval_conseq. Qed.
 
-(** The connection with the rule of consequence is, again, not
-    totally obvious. Recall the rule of consequence for triples.
+(** Here again, the connection with the corresponding reasoning rule for triples
+    is not totally obvious. Recall the statement of the rule of consequence.
 
     triple t H1 Q1 ->
     H2 ==> H1 ->
     Q1 ===> Q2 ->
     triple t H2 Q2
 
-    Let us replace the form [triple t H Q] with the form [H ==> wp t Q].
-    We obtain the following statement: *)
+    Let us replace the form [triple t H Q] with the form [H ==> wp t Q]. We
+    obtain the following statement: *)
 
 Lemma wp_conseq_trans : forall t H1 H2 Q1 Q2,
   H1 ==> wp t Q1 ->
@@ -163,8 +180,8 @@ Lemma wp_conseq_trans : forall t H1 H2 Q1 Q2,
   Q1 ===> Q2 ->
   H2 ==> wp t Q2.
 
-(** If we exploit transitivity of entailment to eliminate [H1] and [H2],
-    then we obtain exactly [wp_conseq], as illustrated below. *)
+(** If we exploit transitivity of entailment to eliminate [H1] and [H2], then we
+    obtain exactly [wp_conseq], as illustrated by the proof script below. *)
 
 Proof using.
   introv M WH WQ. xchange WH. xchange M. applys wp_conseq WQ.
@@ -173,11 +190,10 @@ Qed.
 (* ----------------------------------------------------------------- *)
 (** *** The Extraction Rules *)
 
-(** The extraction rules [triple_hpure] and [triple_hexists]
-    have no specific counterpart with the [wp] presentation.
-    Indeed, in a weakest-precondition style presentation, the
-    extraction rules for triples correspond exactly to the
-    extraction rules for entailment.
+(** The extraction rules [triple_hpure] and [triple_hexists] have no specific
+    counterpart with the [wp] presentation. Indeed, in a weakest-precondition
+    style presentation, the extraction rules for triples correspond exactly to
+    the extraction rules for entailment.
 
     To see why, consider for example the rule [triple_hpure]. *)
 
@@ -185,26 +201,78 @@ Parameter triple_hpure : forall t (P:Prop) H Q,
   (P -> triple t H Q) ->
   triple t (\[P] \* H) Q.
 
-(** Replacing the form [triple t H Q] with [H ==> wp t Q] yields
-    the following statement. *)
+(** Replacing the form [triple t H Q] with [H ==> wp t Q] yields the following
+    statement. *)
 
 Lemma triple_hpure_with_wp : forall t H Q (P:Prop),
   (P -> (H ==> wp t Q)) ->
   (\[P] \* H) ==> wp t Q.
 
-(** The above implication is just a special case of the extraction
-    lemma for pure facts on the left on an entailment, named
-    [himpl_hstar_hpure_l], and whose statement is as follows.
+(** The above implication is just a special case of the extraction lemma for
+    pure facts on the left on an entailment, named [himpl_hstar_hpure_l], and
+    whose statement is as follows.
 
     (P -> (H ==> H')) ->
     (\[P] \* H) ==> H'.
 
-    Instantiating [H'] with [wp t Q] proves [triple_hpure_with_wp].
-*)
+    Instantiating [H'] with [wp t Q] proves [triple_hpure_with_wp]. *)
 
 Proof using. introv M. applys himpl_hstar_hpure_l M. Qed.
 
 (** A similar reasoning applies to the extraction rule for existentials. *)
+
+(* ----------------------------------------------------------------- *)
+(** *** The Ramified Frame Rule *)
+
+(** Recall the ramified frame rule. *)
+
+Parameter triple_ramified_frame : forall H1 Q1 t H Q,
+  triple t H1 Q1 ->
+  H ==> H1 \* (Q1 \--* Q) ->
+  triple t H Q.
+
+(** The ramified frame rule admits in weakest-precondition style, named
+    [wp_ramified]. This rule admits a concise statement and subsumes all other
+    structural rules of Separation Logic. Its very elegant statement is as
+    follows. *)
+
+Lemma wp_ramified : forall t Q1 Q2,
+  (wp t Q1) \* (Q1 \--* Q2) ==> (wp t Q2).
+Proof using. intros. applys wp_conseq_frame. applys qwand_cancel. Qed.
+
+(** The following reformulation of [wp_ramified] can be more practical to
+    exploit in practice, because it applies to any goal of the form
+    [H ==> wp t Q]. *)
+
+Lemma wp_ramified_trans : forall t H Q1 Q2,
+  H ==> (wp t Q1) \* (Q1 \--* Q2) ->
+  H ==> (wp t Q2).
+Proof using. introv M. xchange M. applys wp_ramified. Qed.
+
+(** **** Exercise: 3 stars, standard, especially useful (wp_conseq_of_wp_ramified)
+
+    Prove that [wp_conseq] is derivable from [wp_ramified]. To that end, prove
+    the statement of [wp_conseq] by using only [wp_ramified] or
+    [wp_ramified_trans], and properties of the entailement relation. *)
+
+Lemma wp_conseq_of_wp_ramified : forall t Q1 Q2,
+  Q1 ===> Q2 ->
+  wp t Q1 ==> wp t Q2.
+Proof using. (* FILL IN HERE *) Admitted.
+
+(** [] *)
+
+(** **** Exercise: 3 stars, standard, especially useful (wp_frame_of_wp_ramified)
+
+    Prove that [wp_frame] is derivable from [wp_ramified]. To that end, prove
+    the statement of [wp_frame] by using only [wp_ramified] and properties of
+    the entailement relation. *)
+
+Lemma wp_frame_of_wp_ramified : forall t H Q,
+  (wp t Q) \* H ==> wp t (Q \*+ H).
+Proof using. (* FILL IN HERE *) Admitted.
+
+(** [] *)
 
 (* ================================================================= *)
 (** ** Reasoning Rules for Terms, in Weakest-Precondition Style *)
@@ -212,8 +280,8 @@ Proof using. introv M. applys himpl_hstar_hpure_l M. Qed.
 (* ----------------------------------------------------------------- *)
 (** *** Rule for Values *)
 
-(** Recall the rule [triple_val] which gives a reasoning rule for
-    establishing a triple for a value [v]. *)
+(** Recall the rule [triple_val] which gives a reasoning rule for establishing a
+    triple for a value [v]. *)
 
 Parameter triple_val : forall v H Q,
   H ==> Q v ->
@@ -224,26 +292,14 @@ Parameter triple_val : forall v H Q,
     H ==> Q v ->
     H ==> wp (trm_val v) Q.
 
-    By exploiting transitivity of entailment, we can eliminate [H].
-    We obtain the following statement, which reads as follows:
-    if you own a state satisfying [Q v], then you own a state
-    from which the evaluation of the value [v] produces [Q].
-*)
+    By exploiting transitivity of entailment, we can eliminate [H]. We obtain
+    the following statement, which reads as follows: if you own a state
+    satisfying [Q v], then you own a state from which the evaluation of the
+    value [v] produces [Q]. *)
 
 Lemma wp_val : forall v Q,
   Q v ==> wp (trm_val v) Q.
-Proof using.
-  intros. rewrite wp_equiv. applys* triple_val.
-Qed.
-
-(** We can verify that, when migrating to the [wp] presentation, we have
-    not lost any expressiveness. To that end, we prove that [triple_val] is
-    derivable from [wp_val]. *)
-
-Lemma triple_val_derived_from_wp_val : forall v H Q,
-  H ==> Q v ->
-  triple (trm_val v) H Q.
-Proof using. introv M. rewrite <- wp_equiv. xchange M. applys wp_val. Qed.
+Proof using. unfold wp. intros. intros h K. applys* eval_val. Qed.
 
 (* ----------------------------------------------------------------- *)
 (** *** Rule for Sequence *)
@@ -255,8 +311,8 @@ Parameter triple_seq : forall t1 t2 H Q H1,
   triple t2 H1 Q ->
   triple (trm_seq t1 t2) H Q.
 
-(** Replacing [triple t H Q] with [H ==> wp t Q] throughout the rule
-    gives the statement below.
+(** Replacing [triple t H Q] with [H ==> wp t Q] throughout the rule gives the
+    statement below.
 
       H ==> (wp t1) (fun v => H1) ->
       H1 ==> (wp t2) Q ->
@@ -265,46 +321,38 @@ Parameter triple_seq : forall t1 t2 H Q H1,
     This entailment holds for any [H] and [H1]. Let us specialize it to
     [H1 := (wp t2) Q] and [H := (wp t1) (fun v => (wp t2) Q)].
 
-    This leads us to the following statement, which reads as follows:
-    if you own a state from which the evaluation of [t1] produces a
-    state from which the evaluation of [t2] produces the postcondition
-    [Q], then you own a state from which the evaluation of the sequence
-    [t1;t2] produces [Q]. *)
+    This leads us to the following statement, which reads as follows: if you own
+    a state from which the evaluation of [t1] produces a state from which the
+    evaluation of [t2] produces the postcondition [Q], then you own a state from
+    which the evaluation of the sequence [t1;t2] produces [Q]. *)
 
 Lemma wp_seq : forall t1 t2 Q,
   wp t1 (fun v => wp t2 Q) ==> wp (trm_seq t1 t2) Q.
-Proof using.
-  intros. rewrite wp_equiv. applys triple_seq.
-  { rewrite* <- wp_equiv. }
-  { rewrite* <- wp_equiv. }
-Qed.
+Proof using. unfold wp. intros. intros h K. applys* eval_seq. Qed.
 
-(** **** Exercise: 2 stars, standard, optional (triple_seq_from_wp_seq)
+(* ----------------------------------------------------------------- *)
+(** *** Rule for Let-Bindings *)
 
-    Check that [wp_seq] is just as expressive as [triple_seq],
-    by proving that [triple_seq] is derivable from [wp_seq]
-    and from the structural rules for [wp] and/or the structural
-    rules for [triple]. *)
+(** Recall the reasoning rule for a term [trm_let x t1 t2]. *)
 
-Lemma triple_seq_from_wp_seq : forall t1 t2 H Q H1,
-  triple t1 H (fun v => H1) ->
-  triple t2 H1 Q ->
-  triple (trm_seq t1 t2) H Q.
-Proof using. (* FILL IN HERE *) Admitted.
+Parameter triple_let : forall x t1 t2 Q1 H Q,
+  triple t1 H Q1 ->
+  (forall v1, triple (subst x v1 t2) (Q1 v1) Q) ->
+  triple (trm_let x t1 t2) H Q.
 
-(** [] *)
+(** The rule of [trm_let x t1 t2] is very similar to that for [trm_seq], the
+    only difference being the substitution of [x] by [v] in [t2], where [v]
+    denotes the result of [t1]. *)
 
-(* ################################################################# *)
-(** * More Details *)
-
-(* ================================================================= *)
-(** ** Other Reasoning Rules for Terms *)
+Lemma wp_let : forall x t1 t2 Q,
+  wp t1 (fun v1 => wp (subst x v1 t2) Q) ==> wp (trm_let x t1 t2) Q.
+Proof using. unfold wp. intros. intros h K. applys* eval_let. Qed.
 
 (* ----------------------------------------------------------------- *)
 (** *** Rule for Functions *)
 
-(** Recall the reasoning rule for a term [trm_fun x t1],
-    which evaluates to the value [val_fun x t1]. *)
+(** Recall the reasoning rule for a term [trm_fun x t1], which evaluates to the
+    value [val_fun x t1]. *)
 
 Parameter triple_fun : forall x t1 H Q,
   H ==> Q (val_fun x t1) ->
@@ -314,13 +362,13 @@ Parameter triple_fun : forall x t1 H Q,
 
 Lemma wp_fun : forall x t Q,
   Q (val_fun x t) ==> wp (trm_fun x t) Q.
-Proof using. intros. rewrite wp_equiv. applys* triple_fun. Qed.
+Proof using. unfold wp. intros. intros h K. applys* eval_fun. Qed.
 
 (** A similar rule holds for the evaluation of a recursive function. *)
 
 Lemma wp_fix : forall f x t Q,
   Q (val_fix f x t) ==> wp (trm_fix f x t) Q.
-Proof using. intros. rewrite wp_equiv. applys* triple_fix. Qed.
+Proof using. unfold wp. intros. intros h K. applys* eval_fix. Qed.
 
 (* ----------------------------------------------------------------- *)
 (** *** Rule for Conditionals *)
@@ -340,37 +388,26 @@ Parameter triple_if : forall b t1 t2 H Q,
 
     wp (if b then t1 else t2) Q ==> wp (trm_if (val_bool b) t1 t2) Q.
 
-    This statement corresponds to the wp-style reasoning rule
-    for conditionals. The proof appears next.
-*)
+    This statement corresponds to the wp-style reasoning rule for conditionals.
+    The proof appears next. *)
 
 Lemma wp_if : forall b t1 t2 Q,
   wp (if b then t1 else t2) Q ==> wp (trm_if (val_bool b) t1 t2) Q.
-Proof using.
-  intros. rewrite wp_equiv. applys triple_if. rewrite* <- wp_equiv.
-Qed.
+Proof using. unfold wp. intros. intros h K. applys* eval_if. Qed.
 
-(* ----------------------------------------------------------------- *)
-(** *** Rule for Let-Bindings *)
+(** Equivalently, the rule may be stated with the conditional around the calls
+    to [wp t1 Q] and [wp t2 Q]. *)
 
-(** Recall the reasoning rule for a term [trm_let x t1 t2]. *)
+(** **** Exercise: 1 star, standard, optional (wp_if')
 
-Parameter triple_let : forall x t1 t2 Q1 H Q,
-  triple t1 H Q1 ->
-  (forall v1, triple (subst x v1 t2) (Q1 v1) Q) ->
-  triple (trm_let x t1 t2) H Q.
+    Prove the alternative statement of rule [wp_if], either from [wp_if] or
+    directly from [eval_if]. *)
 
-(** The rule of [trm_let x t1 t2] is very similar to that for
-    [trm_seq], the only difference being the substitution of
-    [x] by [v] in [t2], where [v] denotes the result of [t1]. *)
+Lemma wp_if' : forall b t1 t2 Q,
+  (if b then (wp t1 Q) else (wp t2 Q)) ==> wp (trm_if b t1 t2) Q.
+Proof using. (* FILL IN HERE *) Admitted.
 
-Lemma wp_let : forall x t1 t2 Q,
-  wp t1 (fun v1 => wp (subst x v1 t2) Q) ==> wp (trm_let x t1 t2) Q.
-Proof using.
-  intros. rewrite wp_equiv. applys triple_let.
-  { rewrite* <- wp_equiv. }
-  { intros v. rewrite* <- wp_equiv. }
-Qed.
+(** [] *)
 
 (* ----------------------------------------------------------------- *)
 (** *** Rule For Function Applications *)
@@ -387,180 +424,17 @@ Parameter triple_app_fun : forall x v1 v2 t1 H Q,
 Lemma wp_app_fun : forall x v1 v2 t1 Q,
   v1 = val_fun x t1 ->
   wp (subst x v2 t1) Q ==> wp (trm_app v1 v2) Q.
-Proof using.
-  introv EQ1. rewrite wp_equiv. applys* triple_app_fun.
-  rewrite* <- wp_equiv.
-Qed.
+Proof using. unfold wp. intros. intros h K. applys* eval_app_fun. Qed.
 
 (** A similar rule holds for the application of a recursive function. *)
 
+Lemma wp_app_fix : forall f x v1 v2 t1 Q,
+  v1 = val_fix f x t1 ->
+  wp (subst x v2 (subst f v1 t1)) Q ==> wp (trm_app v1 v2) Q.
+Proof using. unfold wp. intros. intros h K. applys* eval_app_fix. Qed.
+
 (* ################################################################# *)
-(** * Optional Material *)
-
-(* ================================================================= *)
-(** ** A Concrete Definition for Weakest Precondition *)
-
-Module WpHighLevel.
-
-(** The lemma [wp_equiv] captures the characteristic property of [wp],
-    that is, [ (H ==> wp t Q) <-> (triple t H Q) ].
-
-    However, it does not give evidence that there exists a predicate [wp]
-    satisfying this equivalence. We next present one possible definition.
-
-    The idea is to define [wp t Q] as the predicate
-    [\exists H, H \* \[triple t H Q]], which, reading litterally, is
-    satisfied by "any" heap predicate [H] which is a valid precondition
-    for a triple for the term [t] and the postcondition [Q]. *)
-
-Definition wp (t:trm) (Q:val->hprop) : hprop :=
-  \exists (H:hprop), H \* \[triple t H Q].
-
-(** First, let us prove that [wp t Q] is itself a valid precondition,
-    in the sense that [triple t (wp t Q) Q] always holds (as asserted
-    by the lemma [wp_pre]).
-
-    To establish this fact, we have to prove:
-    [triple t (\exists H, H \* \[triple t H Q]) Q].
-
-    Applying the extraction rule for existentials gives:
-    [forall H, triple t (H \* \[triple t H Q]) Q].
-
-    Applying the extraction rule for pure facts gives:
-    [forall H, (triple t H Q) -> (triple t H Q)], which is true. *)
-
-(** Second, let us demonstrate that the heap predicate [wp t Q]
-    is entailed by any precondition [H] that satisfies [triple t H Q],
-    as asserted by the lemma [wp_weakest].
-
-    Assume [triple t H Q]. Let us prove [H ==> wp t Q], that is
-    [H ==> \exists H, H \* \[triple t H Q]]. Instantiating the
-    [H] on the right-hand side as the [H] from the left-hand side
-    suffices to satisfy the entailment. *)
-
-(** Recall that the properties [wp_pre] and [wp_weakest] were derivable
-    from the characteristic equivalence [triple t H Q <-> H ==> wp Q].
-    Thus, to formalize the proofs of [wp_pre] and [wp_weakest], all we
-    have to do is to establish that equivalence. *)
-
-(** **** Exercise: 2 stars, standard, especially useful (wp_equiv)
-
-    Prove that the definition [wp] satisfies the characteristic equivalence
-    for weakest preconditions. *)
-
-Lemma wp_equiv : forall t H Q,
-  (H ==> wp t Q) <-> (triple t H Q).
-Proof using. (* FILL IN HERE *) Admitted.
-
-(** [] *)
-
-End WpHighLevel.
-
-(* ================================================================= *)
-(** ** Equivalence Between all Definitions Of [wp] *)
-
-(** We next prove that the equivalence [(triple t H Q) <-> (H ==> wp t Q)]
-    defines a unique predicate [wp]. In other words, all possible
-    definitions of [wp] are equivalent to each another.
-    Thus, it really does not matter which concrete definition
-    of [wp] we consider: they are all equivalent.
-
-    Concretely, assume two predicates [wp1] and [wp2] to both satisfy
-    the characteristic equivalence. We prove that they are equal. *)
-
-Lemma wp_unique : forall wp1 wp2,
-  (forall t H Q, (triple t H Q) <-> (H ==> wp1 t Q)) ->
-  (forall t H Q, (triple t H Q) <-> (H ==> wp2 t Q)) ->
-  wp1 = wp2.
-Proof using.
-  introv M1 M2. applys fun_ext_2. intros t Q. applys himpl_antisym.
-  { rewrite <- M2. rewrite M1. auto. }
-  { rewrite <- M1. rewrite M2. auto. }
-Qed.
-
-(** Recall that both [wp_pre] and [wp_weakest] are derivable from
-    [wp_equiv]. Let us also that, reciprocally, [wp_equiv] is derivable
-    from the conjunction of [wp_pre] and [wp_weakest].
-
-    In other words, the property of "being the weakest precondition"
-    also uniquely characterizes the definition of [wp]. *)
-
-Lemma wp_from_weakest_pre : forall wp',
-  (forall t Q, triple t (wp' t Q) Q) ->  (* [wp_pre] *)
-  (forall t H Q, triple t H Q -> H ==> wp' t Q) ->  (* [wp_weakest] *)
-  (forall t H Q, H ==> wp' t Q <-> triple t H Q). (* [wp_equiv] *)
-Proof using.
-  introv M1 M2. iff M.
-  { applys triple_conseq M1 M. auto. }
-  { applys M2. auto. }
-Qed.
-
-(* ================================================================= *)
-(** ** An Alternative Definition for Weakest Precondition *)
-
-Module WpLowLevel.
-
-(** The concrete definition for [wp] given above is expressed
-    in terms of Separation Logic combinators. In contrast to
-    this "high level" definition, there exists a more "low level"
-    definition, expressed directly as a function over heaps.
-
-    In that alternative definition, the heap predicate [wp t Q]
-    is defined as a predicate that holds of a heap [h]
-    if and only if the execution of [t] starting in exactly
-    the heap [h] produces the post-condition [Q].
-
-    Technically, [wp t Q] can be defined as:
-    [fun (h:heap) => triple t (fun h' => h' = h) Q].
-    In other words, the precondition requires the input heap
-    to be exactly [h]. *)
-
-Definition wp (t:trm) (Q:val->hprop) : hprop :=
-  fun (h:heap) => triple t (fun h' => (h' = h)) Q.
-
-(** **** Exercise: 4 stars, standard, optional (wp_equiv_wp_low)
-
-    Prove this alternative definition of [wp] also satisfies the
-    characteristic equivalence [H ==> wp Q <-> triple t H Q].
-    Hint: exploit the lemma [triple_named_heap] which was
-    established as an exercise in the appendix of the chapter
-    [Himpl].) *)
-
-Lemma wp_equiv_wp_low : forall t H Q,
-  (H ==> wp t Q) <-> (triple t H Q).
-Proof using. (* FILL IN HERE *) Admitted.
-
-(** [] *)
-
-End WpLowLevel.
-
-(* ================================================================= *)
-(** ** Extraction Rule for Existentials *)
-
-(** Recall the extraction rule for existentials. *)
-
-Parameter triple_hexists : forall t (A:Type) (J:A->hprop) Q,
-  (forall x, triple t (J x) Q) ->
-  triple t (\exists x, J x) Q.
-
-(** Replacing [triple t H Q] with [H ==> wp t Q] yields the
-    lemma stated below. *)
-
-(** **** Exercise: 1 star, standard, optional (triple_hexists_in_wp)
-
-    Prove the extraction rule for existentials in [wp] style. *)
-
-Lemma triple_hexists_in_wp : forall t Q A (J:A->hprop),
-  (forall x, (J x ==> wp t Q)) ->
-  (\exists x, J x) ==> wp t Q.
-
-Proof using. (* FILL IN HERE *) Admitted.
-
-(** [] *)
-
-(** In other words, in the [wp] presentation, we do not need
-    a specific extraction rule for existentials, because the
-    extraction rule for entailment already does the job. *)
+(** * More Details *)
 
 (* ================================================================= *)
 (** ** Combined Structural Rule *)
@@ -573,13 +447,13 @@ Parameter triple_conseq_frame : forall H2 H1 Q1 t H Q,
   Q1 \*+ H2 ===> Q ->
   triple t H Q.
 
-(** Let us reformulate this rule using [wp], replacing the
-    form [triple t H Q] with the form [H ==> wp t Q]. *)
+(** Let us reformulate this rule using [wp], replacing the form [triple t H Q]
+    with the form [H ==> wp t Q]. *)
 
 (** **** Exercise: 2 stars, standard, especially useful (wp_conseq_frame_trans)
 
-    Prove the combined structural rule in [wp] style.
-    Hint: exploit [wp_conseq_trans] and [wp_frame]. *)
+    Prove the combined structural rule in [wp] style. Hint: exploit
+    [wp_conseq_trans] and [wp_frame]. *)
 
 Lemma wp_conseq_frame_trans : forall t H H1 H2 Q1 Q,
   H1 ==> wp t Q1 ->
@@ -592,15 +466,14 @@ Proof using. (* FILL IN HERE *) Admitted.
 
 (** The combined structural rule for [wp] can actually be stated in a more
     concise way. The rule reads as follows: if you own a state from which the
-    execution of [t] produces (a result and a state satisfying) [Q1] and you
-    own [H], and if you can trade the combination of [Q1] and [H] against [Q2],
-    the you own a piece of state from which the execution of [t] produces
-    [Q2]. *)
+    execution of [t] produces (a result and a state satisfying) [Q1] and you own
+    [H], and if you can trade the combination of [Q1] and [H] against [Q2], the
+    you own a piece of state from which the execution of [t] produces [Q2]. *)
 
 (** **** Exercise: 2 stars, standard, especially useful (wp_conseq_frame)
 
-    Prove the concise version of the combined structural rule
-    in [wp] style. Many proofs are possible. *)
+    Prove the concise version of the combined structural rule in [wp] style.
+    Many proofs are possible. *)
 
 Lemma wp_conseq_frame : forall t H Q1 Q2,
   Q1 \*+ H ===> Q2 ->
@@ -609,202 +482,324 @@ Proof using. (* FILL IN HERE *) Admitted.
 
 (** [] *)
 
+(** Let us reformulate the rule [wp_conseq_frame] using a magic wand. The
+    premise [Q1 \*+ H ===> Q2] can be rewritten as [H ==> (Q1 \--* Q2)]. By
+    replacing [H] with [Q1 \--* Q2] in the conclusion of [wp_conseq_frame], we
+    obtain the ramified rule for [wp].
+
+Lemma wp_ramified : forall t Q1 Q2,
+  (wp t Q1) \* (Q1 \--* Q2) ==> (wp t Q2).
+
+    This explaination suggests how one may have come up with the statement of
+    the ramified frame rule. *)
+
+(* ################################################################# *)
+(** * Optional Material *)
+
 (* ================================================================= *)
-(** ** Alternative Statement of the Rule for Conditionals *)
+(** ** Weakest Preconditions Derived from Triples, a First Route *)
 
-Module WpIfAlt.
+Module WpFromTriple.
 
-(** We have established the following rule for reasoning about
-    conditionals using [wp]. *)
+(** The lemma [wp_equiv] captures the characteristic property of [wp], that is,
+    [(H ==> wp t Q) <-> (triple t H Q)]. The predicate [wp] can be defined in
+    terms of [eval], like [triple]. Interestingly, [wp] may also be defined in
+    terms of [triple]. The idea is to define [wp t Q] as the predicate
+    [\exists H, H \* \[triple t H Q]], which, reading litterally, is satisfied
+    by "any" heap predicate [H] which is a valid precondition for a triple for
+    the term [t] and the postcondition [Q]. *)
 
-Parameter wp_if : forall b t1 t2 Q,
-  wp (if b then t1 else t2) Q ==> wp (trm_if b t1 t2) Q.
+Definition wp_1 (t:trm) (Q:val->hprop) : hprop :=
+  \exists (H:hprop), H \* \[triple t H Q].
 
-(** Equivalently, the rule may be stated with the conditional around
-    the calls to [wp t1 Q] and [wp t2 Q]. *)
+(** **** Exercise: 3 stars, standard, especially useful (wp_equiv_1)
 
-(** **** Exercise: 1 star, standard, optional (wp_if')
+    Prove that the alternative definition [wp_1] satisfies the characteristic
+    equivalence for weakest preconditions. Hint: the proof exploits the
+    consequence rule and the extraction rules. *)
 
-    Prove the alternative statement of rule [wp_if],
-    either from [wp_if] or directly from [triple_if]. *)
-
-Lemma wp_if' : forall b t1 t2 Q,
-  (if b then (wp t1 Q) else (wp t2 Q)) ==> wp (trm_if b t1 t2) Q.
+Lemma wp_equiv_1 : forall t H Q,
+  (H ==> wp_1 t Q) <-> (triple t H Q).
 Proof using. (* FILL IN HERE *) Admitted.
 
 (** [] *)
 
-End WpIfAlt.
+End WpFromTriple.
 
 (* ================================================================= *)
-(** ** Definition of [wp] Directly from [hoare] *)
+(** ** Weakest Preconditions Derived From Triples, a Second Route *)
 
-(** Let's take a step back and look at our construction of
-    Separation Logic so far.
+Module WpFromTriple2.
 
-    1. We defined Hoare triples ([hoare]) with respect to the big-step
-       judgment ([eval]).
+(** The concrete definition for [wp] given above is expressed in terms of
+    Separation Logic combinators. In contrast to this "high level" definition,
+    there exists a more "low level" definition, expressed directly as a function
+    over heaps. In this alternative definition, the heap predicate [wp t Q] is
+    defined as a predicate that holds of a heap [h] if and only if the execution
+    of [t] starting in exactly the heap [h] produces the post-condition [Q]. The
+    latter statement is formally captured as [triple t (fun h' => h' = h) Q].
+    The low-level definition of [wp] is thus as shown below. *)
 
-    2. We defined Separation Logic triples ([triple]) in terms of
-       Hoare triples ([hoare]), through the definition:
-       \[forall H', hoare t (H \* H') (Q \*+ H')].
+Definition wp_2 (t:trm) (Q:val->hprop) : hprop :=
+  fun (h:heap) => triple t (fun h' => (h' = h)) Q.
 
-    3. We then defined Separation Logic weakest-preconditions ([wp])
-       in terms of Separation Logic triples ([triple]).
+(** **** Exercise: 4 stars, standard, optional (wp_equiv_2)
 
-    Through the construction, we established reasoning rules, first
-    for Hoare triples ([hoare]), then for Separation Logic triples
-    ([triple]), and finally for weakest-preconditions ([wp]).
+    Prove that the low-level definition [wp_2] also satisfies the characteristic
+    equivalence [H ==> wp Q <-> triple t H Q]. Hint: exploit the lemma
+    [triple_named_heap] which was established as an exercise in the chapter
+    [Triples]. *)
 
-    One question that naturally arises is whether there is a more direct
-    route to deriving reasoning rules for weakest preconditions.
-    In other words, can we obtain the same end result through simpler
-    proofs? *)
-
-(** The notion of Hoare triple is a key abstraction that enables conduction
-    further proofs without manipulating heaps (of type [heap]) explicitly.
-    Experiments suggest that it is beneficial to introduce the Hoare
-    logic layer. In other words, it is counterproductive to try and prove
-    Separation Logic reasoning rules, whether for [triple] or for [wp],
-    directly with respect to the evaluation judgment [eval].
-
-    Thus, the only question that remains is whether it would have some
-    interest to derive the reasoning rules for weakest preconditions ([wp])
-    directly from the the reasoning rules for Hoare triples ([hoare]),
-    that is, by bypassing the statement and proofs for the reasoning rules
-    for Separation Logic triples ([triple]).
-
-    In what follows, we show that if one cares only for [wp]-style rules,
-    then the route to deriving them straight from [hoare]-style rules
-    may indeed be somewhat shorter. *)
-
-Module WpFromHoare.
-
-(** Recall the definition of [triple] in terms of [hoare].
-
-    Definition triple (t:trm) (H:hprop) (Q:val->hprop) : Prop :=
-      forall (H':hprop), hoare t (H \* H') (Q \*+ H').
-
-    In what follows, we conduct the proofs by assuming a concrete definition
-    for [wp] that lends itself better to automated proofs. *)
-
-Definition wp (t:trm) := fun (Q:val->hprop) =>
-  \exists H, H \* \[triple t H Q].
-
-(** First, we check the equivalence between [triple t H Q] and [H ==> wp t Q].
-    This proof is the same as [wp_equiv] from the module [WpHighLevel]
-    given earlier in this chapter. *)
-
-Lemma wp_equiv : forall t H Q,
-  (H ==> wp t Q) <-> (triple t H Q).
-Proof using.
-  unfold wp. iff M.
-  { applys* triple_conseq Q M.
-    applys triple_hexists. intros H'.
-    rewrite hstar_comm. applys* triple_hpure. }
-  { xsimpl* H. }
-Qed.
-
-(** Second, we prove the consequence-frame rule associated with [wp].
-    It is the only structural rule that is needed for working with
-    weakest preconditions. *)
-
-Lemma wp_conseq_frame : forall t H Q1 Q2,
-  Q1 \*+ H ===> Q2 ->
-  (wp t Q1) \* H ==> (wp t Q2).
-
-(** The proof leverages the consequence rule for [hoare] triples,
-    and the frame property comes from the [forall H'] quantification
-    baked in the definition of [triple]. *)
-
-Proof using.
-  introv M. unfold wp. xpull. intros H' N. xsimpl (H' \* H).
-  unfolds triple. intros H''. specializes N (H \* H'').
-  applys hoare_conseq N. { xsimpl. } { xchange M. }
-Qed.
-
-(** Third and last, we establish reasoning rules for terms in [wp]-style
-    directly from the corresponding rules for [hoare] triples.
-
-    The proof details are beyond the scope of this course.
-    The point here is to show that the proofs are fairly concise. *)
-
-Lemma wp_val : forall v Q,
-  Q v ==> wp (trm_val v) Q.
-Proof using.
-  intros. unfold wp. xsimpl. intros H'. applys hoare_val. xsimpl.
-Qed.
-
-Lemma wp_fun : forall x t Q,
-  Q (val_fun x t) ==> wp (trm_fun x t) Q.
-Proof using.
-  intros. unfold wp. xsimpl. intros H'. applys hoare_fun. xsimpl.
-Qed.
-
-Lemma wp_fix : forall f x t Q,
-  Q (val_fix f x t) ==> wp (trm_fix f x t) Q.
-Proof using.
-  intros. unfold wp. xsimpl. intros H'. applys hoare_fix. xsimpl.
-Qed.
-
-Lemma wp_if : forall b t1 t2 Q,
-  wp (if b then t1 else t2) Q ==> wp (trm_if b t1 t2) Q.
-Proof using.
-  intros. unfold wp. xsimpl. intros H M H'.
-  applys hoare_if. applys M.
-Qed.
-
-Lemma wp_app_fun : forall x v1 v2 t1 Q,
-  v1 = val_fun x t1 ->
-  wp (subst x v2 t1) Q ==> wp (trm_app v1 v2) Q.
-Proof using.
-  introv EQ1. unfold wp. xsimpl. intros H' M. intros H''. applys* hoare_app_fun.
-Qed.
-
-Lemma wp_app_fix : forall f x v1 v2 t1 Q,
-  v1 = val_fix f x t1 ->
-  wp (subst x v2 (subst f v1 t1)) Q ==> wp (trm_app v1 v2) Q.
-Proof using.
-  introv EQ1. unfold wp. xsimpl. intros H' M. intros H''. applys* hoare_app_fix.
-Qed.
-
-(** **** Exercise: 4 stars, standard, especially useful (wp_let)
-
-    Prove wp-style rule for let bindings. *)
-
-Lemma wp_let : forall x t1 t2 Q,
-  wp t1 (fun v => wp (subst x v t2) Q) ==> wp (trm_let x t1 t2) Q.
+Lemma wp_equiv_2 : forall t H Q,
+  (H ==> wp_2 t Q) <-> (triple t H Q).
 Proof using. (* FILL IN HERE *) Admitted.
 
 (** [] *)
 
-(** Note: [wp_seq] admits essentially the same proof as [wp_let], simply
-    replacing [hoare_let] with [hoare_seq], and removing the tactic
-    [intros v]. *)
+End WpFromTriple2.
 
-(** It is technically possible to bypass even the definition of
-    [triple] and specify all functions directly using the predicate
-    [wp]. However, using [triple] leads to better readability of
-    specifications, thus it seems preferable to continue using that
-    style for specifying functions. (See discussion in chapter
-    [Wand], appendix on "Texan triples".) *)
+(* ================================================================= *)
+(** ** Characterizations of [wp] *)
 
-End WpFromHoare.
+(** First, we establish that the equivalence [(triple t H Q) <-> (H ==> wp t Q)]
+    defines a unique predicate [wp]. In other words, all possible definitions of
+    [wp] are equivalent to each another. Thus, it really does not matter which
+    concrete definition of [wp] we consider: they are all equivalent.
+    Concretely, assume two predicates [wp1] and [wp2] to both satisfy the
+    characteristic equivalence. We prove that they are equal. *)
+
+Lemma wp_unique : forall wp1 wp2,
+  (forall t H Q, (triple t H Q) <-> (H ==> wp1 t Q)) ->
+  (forall t H Q, (triple t H Q) <-> (H ==> wp2 t Q)) ->
+  wp1 = wp2.
+Proof using.
+  introv M1 M2. applys fun_ext_2. intros t Q. applys himpl_antisym.
+  { rewrite <- M2. rewrite M1. auto. }
+  { rewrite <- M1. rewrite M2. auto. }
+Qed.
+
+(** Second, we establish that the property of "being the weakest precondition"
+    also uniquely characterizes the definition of [wp]. This property is the
+    conjunction of two facts: [wp t Q] must be a valid precondition for a triple
+    involving [t] and [Q]; and [wp t Q] must be entailed by any valid
+    precondition of a triple involving [t] and [Q]. These two facts correspond
+    to [wp_pre] and [wp_weakest]. *)
+
+(** **** Exercise: 2 stars, standard, especially useful (wp_equiv_iff_wp_pre_and_wp_weakest)
+
+    Prove that the conjunction of the properties [wp_pre] and [wk_weakest] is
+    equivalent to the property [wp_equiv]. *)
+
+Lemma wp_equiv_iff_wp_pre_and_wp_weakest : forall wp',
+  (   (forall t Q, triple t (wp' t Q) Q) (* [wp_pre] *)
+   /\ (forall t H Q, triple t H Q -> H ==> wp' t Q)) (* [wp_weakest] *)
+  <->
+  (forall t H Q, H ==> wp' t Q <-> triple t H Q). (* [wp_equiv] *)
+Proof using. (* FILL IN HERE *) Admitted.
+
+(** [] *)
+
+
+(* ================================================================= *)
+(** ** Texan Triples *)
+
+Module TexanTriples.
+
+(* ----------------------------------------------------------------- *)
+(** *** 1. Example of Texan Triples *)
+
+(** In this section, we show that specification triples can be presented in a
+    different style using weakest preconditions. Consider for example the
+    specification triple for allocation. *)
+
+Parameter triple_ref : forall v,
+  triple (val_ref v)
+    \[]
+    (funloc p => p ~~> v).
+
+(** This specification may be equivalently reformulated in the form of an
+    entailment, as shown below. Note that we purposely leave an empty heap
+    predicate at the front to indicate where the precondition, if it were not
+    empty, would go in the reformulation. *)
+
+Parameter wp_ref : forall Q v,
+  \[] \* (\forall p, p ~~> v \-* Q (val_loc p)) ==> wp (val_ref v) Q.
+
+(** In what follows, we describe the chain of transformation that can take us
+    from the triple form to the [wp] form, and establish the reciprocal.
+    Afterwards, we will formalize the general pattern of the translation from a
+    triple to a "texan triple", that is, to a wp-based specification. *)
+
+(** By replacing [triple t H Q] with [H ==> wp t Q], the specification
+    [triple_ref] can be reformulated as follows. *)
+
+Lemma wp_ref_0 : forall v,
+  \[] ==> wp (val_ref v) (funloc p => p ~~> v).
+Proof using. intros. rewrite wp_equiv. applys triple_ref. Qed.
+
+(** We wish to cast the RHS in the form [wp (val_ref v) Q] for an abstract
+    postcondition [Q]. To that end, we reformulate the above statement by
+    including a magic wand relating the postcondition [(funloc p => p ~~> v)]
+    with [Q]. *)
+
+Lemma wp_ref_1 : forall Q v,
+  ((funloc p => p ~~> v) \--* Q) ==> wp (val_ref v) Q.
+Proof using. intros. xchange (wp_ref_0 v). applys wp_ramified. Qed.
+
+(** This statement can be made slightly more readable by unfolding the
+    definition of the magic wand for postconditions. Doing so amounts to
+    quantifying explicitly on the result, named [r]. *)
+
+Lemma wp_ref_2 : forall Q v,
+  (\forall r,     (\exists p, \[r = val_loc p] \* p ~~> v) \-* Q r)
+              ==> wp (val_ref v) Q.
+Proof using. intros. applys himpl_trans wp_ref_1. xsimpl. Qed.
+
+(** Interestingly, the variable [r], which is equal to [val_loc p], can now be
+    substituted away, further increasing readability. We obtain the
+    specification of [val_ref] in "Texan triple style". *)
+
+Lemma wp_ref_3 : forall Q v,
+  (\forall p, (p ~~> v) \-* Q (val_loc p)) ==> wp (val_ref v) Q.
+Proof using.
+  intros. applys himpl_trans wp_ref_2. xsimpl. intros ? p ->.
+  xchange (hforall_specialize p).
+Qed.
+
+(* ----------------------------------------------------------------- *)
+(** *** 2. The General Pattern *)
+
+(** Most specification triples can be casted in the form:
+    [triple t H (fun r => exists x1 .. xN, \[r = v] \* H')]. In such a
+    specification:
+
+    - the value [v] may depend on the [xi] variables,
+    - the heap predicate [H'] may depend on [r] and the [xi],
+    - the number of existentials [xi] may vary, possibly be zero,
+    - the equality [\[r = v]] may be removed if no pure fact is needed
+      about [r].
+
+    Such a specification triple of the form
+    [triple t H (fun r => exists x1 xN, \[r = v] \* H'] can be be reformulated
+    as the Texan triple: [(\forall x1 xN, H \-* Q v) ==> wp t Q].
+
+    We next formalize the equivalence between the two presentations, for the
+    specific case where the specification involves a single auxiliary variable,
+    named [x]. The statement below makes it explicit that [v] may depend on [x],
+    and that [H] may depend on [r] and [x]. *)
+
+Lemma texan_triple_equiv : forall t H A (Hof:val->A->hprop) (vof:A->val),
+      (triple t H (fun r => \exists x, \[r = vof x] \* Hof r x))
+  <-> (forall Q, H \* (\forall x, Hof (vof x) x \-* Q (vof x)) ==> wp t Q).
+Proof using.
+  intros. rewrite <- wp_equiv. iff M.
+  { intros Q. xchange M. applys wp_ramified_trans.
+    xsimpl. intros r x ->.
+    xchange (hforall_specialize x). }
+  { applys himpl_trans M. xsimpl~. }
+Qed.
+
+(* ----------------------------------------------------------------- *)
+(** *** 3. Other Examples *)
+
+Section WpSpecRef.
+
+(** The wp-style specification of [ref], [get] and [set] are presented next. *)
+
+Lemma wp_get : forall v p Q,
+  (p ~~> v) \* (p ~~> v \-* Q v) ==> wp (val_get p) Q.
+Proof using.
+  intros. rewrite wp_equiv. applys triple_conseq_frame.
+  { applys triple_get. } { applys himpl_refl. } { xsimpl. intros ? ->. auto. }
+Qed.
+
+Lemma wp_set : forall v w p Q,
+  (p ~~> v) \* (\forall r, p ~~> w \-* Q r) ==> wp (val_set p w) Q.
+Proof using.
+  intros. rewrite wp_equiv. applys triple_conseq_frame.
+  { applys triple_set. } { applys himpl_refl. }
+  { intros r. xchange (hforall_specialize r). xsimpl. }
+Qed.
+
+Lemma wp_free : forall v p Q,
+  (p ~~> v) \* (\forall r, Q r) ==> wp (val_free p) Q.
+Proof using.
+  intros. rewrite wp_equiv. applys triple_conseq_frame.
+  { applys triple_free. } { applys himpl_refl. }
+  { intros r. xchange (hforall_specialize r). }
+Qed.
+
+(** Alternatively, the specifications of [set] and [free] may advertize that the
+    output value is the unit value. *)
+
+Parameter triple_set' : forall w p v,
+  triple (val_set p w)
+    (p ~~> v)
+    (fun r => \[r = val_unit] \* p ~~> w).
+
+Lemma wp_set' : forall v w p Q,
+  (p ~~> v) \* (p ~~> w \-* Q val_unit) ==> wp (val_set p w) Q.
+Proof using.
+  intros. rewrite wp_equiv. applys triple_conseq_frame.
+  { applys triple_set'. }
+  { applys himpl_refl. }
+  { xsimpl. intros ? ->. auto. }
+Qed.
+
+Parameter triple_free' : forall p v,
+  triple (val_free p)
+    (p ~~> v)
+    (fun r => \[r = val_unit]).
+
+Lemma wp_free' : forall v w p Q,
+  (p ~~> v) \* (Q val_unit) ==> wp (val_free p) Q.
+Proof using.
+  intros. rewrite wp_equiv. applys triple_conseq_frame.
+  { applys triple_free'. }
+  { applys himpl_refl. }
+  { xsimpl. intros ? ->. auto. }
+Qed.
+
+End WpSpecRef.
+
+(* ----------------------------------------------------------------- *)
+(** *** 4. Exercise *)
+
+(** Let us put to practice the use of a Texan triple on a different example.
+    Recall the function [incr] and its specification (from [Hprop.v]). *)
+
+Parameter incr : val.
+
+Parameter triple_incr : forall (p:loc) (n:int),
+  triple (incr p)
+    (p ~~> n)
+    (fun v => \[v = val_unit] \* (p ~~> (n+1))).
+
+(** **** Exercise: 3 stars, standard, especially useful (wp_incr)
+
+    State a Texan triple for [incr] as a lemma called [wp_incr], then prove this
+    lemma from [triple_incr]. *)
+
+(* FILL IN HERE *)
+
+(** [] *)
+
+End TexanTriples.
 
 
 (* ================================================================= *)
 (** ** Historical Notes *)
 
-(** The idea of weakest precondition was introduced by [Dijstra 1975] (in Bib.v)
-    in his seminal paper "Guarded Commands, Nondeterminacy and Formal
-    Derivation of Programs".
+(** The idea of weakest precondition was introduced by [Dijstra 1975] (in Bib.v) in
+    his seminal paper "Guarded Commands, Nondeterminacy and Formal Derivation of
+    Programs". Weakest preconditions provide a reformulation of Floyd-Hoare
+    logic. Numerous practical verification tools leverage weakest preconditions,
+    e.g. ESC/Java, Why3, Boogie, Spec#, etc. In the context of Separation Logic
+    in a proof assistant, the Iris framework (https://iris-project.org/),
+    developed since 2015, prevasively exploits weakest preconditions to state
+    reasoning rules. Developers of the tools VST and Iris have advertised for
+    the interest of this rule. The ramified frame rule was integrated in CFML
+    2.0 in 2018. Texan triples have been used in certain Iris-based
+    formalizations. *)
 
-    Weakest preconditions provide a reformulation of Floyd-Hoare logic.
-    Numerous practical verification tools leverage weakest preconditions,
-    e.g. ESC/Java, Why3, Boogie, Spec#, etc.
-
-    In the context of Separation Logic in a proof assistant, the Iris framework
-    (https://iris-project.org/), developed since 2015, exploits weakest
-    preconditions to state reasoning rules. See the [Postscript]. *)
-
-(* 2023-08-23 12:58 *)
+(* 2023-11-29 09:22 *)
