src/slf/LibChoice.v
@@ -215,4 +215,4 @@ Proof using. intros. apply~ guarded_rel_choice. Qed.
 
 
 
-(* 2023-08-23 12:58 *)
+(* 2023-11-29 09:22 *)
