src/slf/LibEqual.v
@@ -922,4 +922,4 @@ Proof using.
   apply~ eq_dep_of_JMeq.
 Qed.
 
-(* 2023-08-23 12:57 *)
+(* 2023-11-29 09:22 *)
