src/slf/LibMin.v
@@ -258,4 +258,4 @@ Definition MMax `{Inhab A} `{Le A} := mmax le.
 
 
 
-(* 2023-08-23 12:58 *)
+(* 2023-11-29 09:22 *)
