src/slf/LibWf.v
@@ -596,4 +596,4 @@ Proof using.
   induction 1; eauto using Acc_inv.
 Qed.
 
-(* 2023-08-23 12:57 *)
+(* 2023-11-29 09:22 *)
