src/slf/LibAxioms.v
@@ -52,4 +52,4 @@ Axiom indefinite_description : forall (A : Type) (P : A->Prop),
   ex P ->
   sig P.
 
-(* 2023-08-23 12:57 *)
+(* 2023-11-29 09:22 *)
